

## *Lecture 2. Math Review (2)*

Sim, Min Kyu, Ph.D.  
mksim@seoultech.ac.kr

## Math Review 17

- For  $X \sim U(20, 40)$ , Evaluate  $\mathbb{E}[X \wedge 25]$  and  $\mathbb{E}[(25 - X)^+]$

## Math Review 18

■ For  $X \sim Poi(8)$ ,

- $\mathbb{P}(X = 0) =$

- $\mathbb{P}(2 \leq X \leq 4) =$

- $\mathbb{P}(X > 2) =$

## Math Review 19

- For  $X \sim \exp(7)$ , Evaluate  $\mathbb{E}[\max(X, 7)]$

## Math Review 20

- For  $X \sim \text{exp}(8)$ , find  $x^*$  such that  $F(x^*) = 0.6$

## Math Review 21

- For  $X \sim U(10, 20)$ , find  $x^*$  such that  $F(x^*) = 0.7$

*blank*

### ■ Matrix Multiplication

$$(.6 \quad .4) \begin{pmatrix} .7 & .3 \\ .5 & .5 \end{pmatrix} =$$



■ Solve

$$(\pi_1 \quad \pi_2) \begin{pmatrix} .7 & .3 \\ .5 & .5 \end{pmatrix} = (\pi_1 \quad \pi_2)$$

$$\pi_1 + \pi_2 = 1$$

- Solve the following system of equations

$$x = y$$

$$y = 0.5z$$

$$z = 0.6 + 0.4x$$

$$x + y + z = 1$$

■ Solve

$$(\pi_0 \quad \pi_1 \quad \pi_2) \begin{pmatrix} -2 & 2 \\ 3 & -5 & 2 \\ & 3 & -3 \end{pmatrix} = (0 \quad 0 \quad 0)$$

$$\pi_0 + \pi_1 + \pi_2 = 1$$

$$P = \begin{pmatrix} .7 & .3 \\ .5 & .5 \end{pmatrix}$$

- What is  $P^2$  ?

■ Solve

$$(\pi_1 \quad \pi_2 \quad \pi_3 \quad \pi_4) \begin{pmatrix} .7 & .3 & & \\ .5 & .5 & & \\ & & .6 & .4 \\ & & .3 & .7 \end{pmatrix} = (\pi_1 \quad \pi_2 \quad \pi_3 \quad \pi_4)$$

$$\pi_1 + \pi_2 + \pi_3 + \pi_4 = 1$$

*blank*

## Math Review 23 - Express infinite vector math form

- Solve the following and express  $\pi_i$  for  $i = 0, 1, 2, \dots$

$$\begin{aligned}\pi_0 + \pi_1 + \pi_2 + \dots &= 1 \\ 0.02\pi_0 + 0.02\pi_1 + 0.02\pi_2 + \dots &= \pi_0 \\ 0.98\pi_0 &= \pi_1 \\ 0.98\pi_1 &= \pi_2 \\ 0.98\pi_2 &= \pi_3 \\ \dots &= \dots\end{aligned}$$

*blank*



## *Math Review 24 - Infinite Geometric Series*

- When  $|r| < 1$ ,  $S = a + ar + ar^2 + ar^3 + \dots$

## Math Review 25 - Geometric Series

- When  $r \neq 1$ ,  $S = a + ar + ar^2 + ar^3 + \dots + ar^{n-1}$

## *Math Review 26 - Power Series*

- When  $|r| < 1$ ,  $S = r + 2r^2 + 3r^3 + 4r^4 + \dots$

*blank*

## *Math Review 27 - Conditional Probabilities*

- Show that  $\mathbb{P}(A|B \cap C)\mathbb{P}(B|C) = \mathbb{P}(A \cap B|C)$

*blank*

## *Math Review 28 - Formulation of time varying function*

- During the first hour ( $0 \leq t \leq 1$ ),  $\lambda(t)$  increases linearly from 0 to 60. After the first hour,  $\lambda(t)$  is constant at 60. Draw plot for  $\lambda(t)$  and express the function in math form.

*blank*



## Exercise 1

- For  $X \sim U(a, b)$ , show pdf  $\rightarrow$  cdf

## Exercise 2

- For  $X \sim \exp(\lambda)$ , what is pdf  $f(x)$ ?

### Exercise 3

- For  $X \sim \exp(\lambda)$ , show pdf  $\rightarrow$  cdf.

## Exercise 4

- For  $X \sim \exp(\lambda)$ , show that  $\mathbb{E}X = 1/\lambda$

## Exercise 5

- For  $X \sim \text{exp}(\lambda)$ , show that  $\text{Var}(X) = 1/\lambda^2$
- (hint) (You may prove this by continuing the following:)

pf) Since  $\text{Var}(X) = \mathbb{E}X^2 - (\mathbb{E}X)^2$  and we know  $\mathbb{E}X = 1/\lambda$  from **hw1.#4**, we need to know what  $\mathbb{E}X^2$  is.

$$\begin{aligned}\mathbb{E}X^2 &= \int_{-\infty}^{\infty} x^2 f(x) dx = \int_0^{\infty} x^2 \lambda e^{-\lambda x} dx = \lambda \int_0^{\infty} x^2 e^{-\lambda x} dx \\ &= \lambda \left( x^2 \cdot -\frac{1}{\lambda} e^{-\lambda x} \Big|_0^{\infty} - \int_0^{\infty} 2x \cdot -\frac{1}{\lambda} e^{-\lambda x} dx \right) \\ &= \dots\end{aligned}$$

■ Solution

$$\begin{aligned} &= \lambda \left( (0 - 0) + \frac{2}{\lambda} \int_0^{\infty} x e^{-\lambda x} dx \right) = 2 \int_0^{\infty} x e^{-\lambda x} dx \\ &= 2 \left[ x \cdot -\frac{1}{\lambda} e^{-\lambda x} \Big|_0^{\infty} - \int_0^{\infty} -\frac{1}{\lambda} e^{-\lambda x} dx \right] \\ &= 2 \left[ \infty \cdot -\frac{1}{\lambda} e^{-\lambda \infty} - \left( 0 \cdot -\frac{1}{\lambda} e^{-\lambda 0} \right) + \frac{1}{\lambda} \left[ -\frac{1}{\lambda} e^{-\lambda x} \right]_0^{\infty} \right] \\ &= 2 \left[ 0 - 0 + \frac{1}{\lambda} \left[ -\frac{1}{\lambda} e^{-\lambda \infty} + \frac{1}{\lambda} e^{-\lambda 0} \right] \right] \\ &= 2 \cdot \frac{1}{\lambda} \left( 0 + \frac{1}{\lambda} \right) = \frac{2}{\lambda^2} \end{aligned}$$

Since  $Var(x) = \mathbb{E}X^2 - (\mathbb{E}X)^2$ ,  $Var(x) = \frac{2}{\lambda^2} - \left(\frac{1}{\lambda}\right)^2 = \frac{1}{\lambda^2}$

## Exercise 6

- Show that Exponential distribution is memoryless.

## Exercise 7

- For  $X \sim \text{Poi}(\lambda)$ , show that  $\mathbb{E}X = \lambda$



## Exercise 8

■ For  $X \sim \text{Poi}(\lambda)$ , show that  $\text{Var}(X) = \lambda$

■ (hint) (you may prove by continuing following.)

pf) Since  $\text{Var}(X) = \mathbb{E}X^2 - (\mathbb{E}X)^2$  and we know  $\mathbb{E}X = \lambda$  from **hw1.#7**, we need to know what  $\mathbb{E}X^2$  is.

$$\begin{aligned}\mathbb{E}X^2 &= \sum_{x=-\infty}^{\infty} x^2 p(x) = \sum_{x=0}^{\infty} x^2 \frac{\lambda^x e^{-\lambda}}{x!} = e^{-\lambda} \sum_{x=0}^{\infty} x^2 \frac{\lambda^x}{x!} \\&= e^{-\lambda} \left( 0^2 \frac{\lambda^0}{0!} + \sum_{x=1}^{\infty} x^2 \frac{\lambda^x}{x!} \right) \\&= e^{-\lambda} \left( \sum_{x=1}^{\infty} x \frac{\lambda^x}{(x-1)!} \right) \\&= e^{-\lambda} \left( \sum_{x=1}^{\infty} (x-1+1) \frac{\lambda^x}{(x-1)!} \right) \\&= e^{-\lambda} \left( \sum_{x=1}^{\infty} (x-1) \frac{\lambda^x}{(x-1)!} + \sum_{x=1}^{\infty} \frac{\lambda^x}{(x-1)!} \right) \\&= e^{-\lambda} \left( \sum_{x=2}^{\infty} \frac{\lambda^x}{(x-2)!} + \sum_{x=1}^{\infty} \frac{\lambda^x}{(x-1)!} \right) \\&= \dots\end{aligned}$$

## ■ Solution

$$\begin{aligned} &= e^{-\lambda} \left[ \lambda^2 \sum_{x=2}^{\infty} \frac{\lambda^{x-2}}{(x-2)!} + \lambda \sum_{x=1}^{\infty} \frac{\lambda^{x-1}}{(x-1)!} \right] \\ &= e^{-\lambda} \left[ \lambda^2 \sum_{y=0}^{\infty} \frac{\lambda^y}{y!} + \lambda \sum_{z=0}^{\infty} \frac{\lambda^z}{z!} \right], \text{ where } y := x-2, z := x-1 \\ &= e^{-\lambda} [\lambda^2 \cdot e^{\lambda} + \lambda \cdot e^{\lambda}] \\ &= \lambda^2 + \lambda \end{aligned}$$

$$\text{Var}(x) = \mathbb{E}X^2 - (\mathbb{E}X)^2 = \lambda^2 + \lambda - \lambda^2 = \lambda$$

(Note that the property of exponential function is used, i.e.  $e^x = \sum_{i=0}^{\infty} \frac{x^i}{i!}$ )

## Exercise 9

- Let  $X$  be a discrete random variable with  $\mathbb{P}(X = i) = ci$  for positive, odd integers  $i < 8$ ; otherwise, the probability is zero.
- (a) Compute the value of  $c$ . (by using the one of the properties of pmf)
  - (b) What is the mean of  $X$ ?
  - (c) What is the second moment of  $X$ ? (i.e. What is  $\mathbb{E}X^2$ ?)
  - (d) What is the variance of  $X$ ?
  - (e) Compute  $\mathbb{E}[(X - 3)^+]$

## ■ Solution

(a) Since  $\sum_{i=-\infty}^{\infty} p(i) = \sum_{i=-\infty}^{\infty} \mathbb{P}(X = i) = 1,$

$$\mathbb{P}(X = 1) + \mathbb{P}(X = 3) + \mathbb{P}(X = 5) + \mathbb{P}(X = 7) = c + 3c + 5c + 7c = 1$$

$$\therefore c = 1/16$$

(b)

$$\begin{aligned}\mathbb{E}X &= \sum_{i=-\infty}^{\infty} i \cdot p(i) = \sum_{i=-\infty}^{\infty} i \cdot \mathbb{P}(X = i) = 1 \cdot p(1) + 3 \cdot p(3) + 5 \cdot p(5) + 7 \cdot p(7) \\ &= \frac{1}{16}(1^2 + 3^2 + 5^2 + 7^2) = \frac{84}{16} = \frac{21}{4}\end{aligned}$$

(c)

$$\begin{aligned}\mathbb{E}X^2 &= \sum_{i=-\infty}^{\infty} i^2 \cdot p(i) = \sum_{i=-\infty}^{\infty} i^2 \cdot \mathbb{P}(X = i) = 1^2 \cdot p(1) + 3^2 \cdot p(3) + 5^2 \cdot p(5) + 7^2 \cdot p(7) \\ &= \frac{1}{16}(1^3 + 3^3 + 5^3 + 7^3) = \frac{496}{16} = \frac{124}{4} = 31\end{aligned}$$

$$(d) \operatorname{Var}(X) = \mathbb{E}X^2 - (\mathbb{E}X)^2 = 31 - \left(\frac{21}{4}\right)^2 = 3.4375$$

(e)

$$\begin{aligned}\mathbb{E}[(X-3)^+] &= \mathbb{E}[\max(X-3, 0)] = \sum_{i=-\infty}^{\infty} \max(i-3, 0) \cdot \mathbb{P}(X=i) \\&= \max(1-3, 0) \cdot \mathbb{P}(X=1) + \max(3-3, 0) \cdot \mathbb{P}(X=3) \\&\quad + \max(5-3, 0) \cdot \mathbb{P}(X=5) + \max(7-3, 0) \cdot \mathbb{P}(X=7) \\&= 2 \cdot \frac{5}{16} + 4 \cdot \frac{7}{16} = \frac{38}{16} = \frac{19}{8}\end{aligned}$$

## Exercise 10

- Let  $X$  be a Poisson random variable with parameter 5, and let  $Y = \min(X, 2)$
- (a) What is the pmf of  $X$ ?
  - (b) What is the mean of  $X$ ?
  - (c) What is the variance of  $X$ ?
  - (d) What is the pmf of  $Y$ ? (i.e. Specify  $\mathbb{P}(Y = i)$  for  $i = 0, 1, 2, \dots$ )
  - (e) Compute  $E[Y]$ ?

■ Solution

(a)  $p(x) = \mathbb{P}(X = x) = \frac{e^{-5}5^x}{x!}$

(b) 5 ( $= \lambda$ )

(c) 5 ( $= \lambda$ )

(d) We have  $p(y) = \mathbb{P}(Y = y) = \mathbb{P}(\min(X, 2) = y)$ . It follows:

■  $p(0) = \mathbb{P}(Y = 0) = \mathbb{P}(\min(X, 2) = 0) = \mathbb{P}(X = 0) = \frac{e^{-5}5^0}{0!} = e^{-5}$

■  $p(1) = \mathbb{P}(Y = 1) = \mathbb{P}(\min(X, 2) = 1) = \mathbb{P}(X = 1) = \frac{e^{-5}5^1}{1!} = 5e^{-5}$

■  $p(2) = \mathbb{P}(Y = 2) = \mathbb{P}(\min(X, 2) = 2) = \mathbb{P}(X \geq 2) = 1 - \mathbb{P}(X = 0) - \mathbb{P}(X = 1) = 1 - e^{-5} - 5e^{-5} = 1 - 6e^{-5}$

■  $p(3) = \mathbb{P}(Y = 3) = 0$  ( $\because \min(X, 2) \leq 2$  always), also  $p(i) = 0$  for all  $i \geq 3$

■ Therefore,

$$p(y) = \begin{pmatrix} e^{-5} \text{ for } y = 0 \\ 5e^{-5} \text{ for } y = 1 \\ 1 - 6e^{-5} \text{ for } y \geq 2 \end{pmatrix}$$

(e)

$$\mathbb{E}Y = \sum_{i=-\infty}^{\infty} yp(y) = 0 \cdot p(0) + 1 \cdot p(1) + 2 \cdot p(2) = 5e^{-5} + 2(1 - 6e^{-5}) = 2 - 7e^{-5}$$



## Exercise 11

- Let  $Y$  be a random variable with pdf  $ce^{-3y}$  for  $y > 0$ , and zero otherwise.
- (a) Determine  $c$ .
  - (b) What is the mean, variance, and squared coefficient of variation of  $Y$ ?
  - (c) Compute  $\mathbb{P}(Y > 4)$
  - (d) Compute  $\mathbb{P}(Y > 7 | Y > 3)$
  - (e) Your answer for (c) and answer for (d) should be same. Discuss shortly why.
  - (f) What is the point  $x^*$  such that  $\mathbb{P}(Y > x^*) = 2/3$ ?

## ■ Solution

(a)

$$\int_{-\infty}^{\infty} p(y) dy = 1$$

$$\rightarrow \int_0^{\infty} ce^{-3y} dy = c \cdot -\frac{1}{3} e^{-3y} \Big|_0^{\infty} = -\frac{c}{3} [0 - e^{-3 \cdot 0}] = \frac{c}{3} = 1$$

$$\therefore c = 3$$

(b) pdf of  $\begin{cases} 3e^{-3y} & y \geq 0 \\ 0 & \text{otherwise} \end{cases}$  implies  $Y \sim \exp(3)$ . Thus,  $\mathbb{E}Y = \frac{1}{3}$ ,  $VarY = \frac{1}{3^2}$ ,  
and  $\text{sqr-cv} = \frac{Var(Y)}{(\mathbb{E}Y)^2} = \frac{1/3^2}{(1/3)^2} = 1$

(c) cdf of  $\exp(3)$  is  $\begin{cases} 1 - e^{-3y} & \text{for } y \geq 0 \\ 0 & \text{otherwise} \end{cases}$  Thus,

$$\mathbb{P}(Y > 4) = 1 - \mathbb{P}(Y \leq 4) = 1 - (1 - e^{-3 \cdot 4}) = e^{-12}$$

$$(d) \mathbb{P}(Y > 7 | Y > 3) = \frac{\mathbb{P}(Y > 7, Y > 3)}{\mathbb{P}(Y > 3)} = \frac{1 - (1 - e^{-3 \cdot 7})}{1 - (1 - e^{-3 \cdot 3})} = \frac{e^{-21}}{e^{-9}} = e^{-12}$$

(e) memoryless property

(f)

$$\mathbb{P}(Y > x^*) = 1 - \mathbb{P}(Y \leq x^*) = 1 - (1 - e^{-3x^*}) = \frac{2}{3}$$

$$\rightarrow e^{-3x^*} = \frac{2}{3}$$

$$\rightarrow -3x^* = \ln(2/3)$$

$$\rightarrow x^* = -\frac{1}{3} \ln(2/3)$$

*blank*

"Man can learn nothing unless he proceeds from the known to the unknown."  
- Claude Bernard"